the first fully-building Rtac in a while.

theories/RTac/Apply.v
@@ -4,6 +4,7 @@ Require Import MirrorCore.ExprDAs.
 Require Import MirrorCore.Lemma.
 Require Import MirrorCore.LemmaApply.
 Require Import MirrorCore.InstantiateI.
+Require Import MirrorCore.VariablesI.
 Require Import MirrorCore.RTac.Core.
 Require Import MirrorCore.RTac.Reduce.
 Require Import MirrorCore.RTac.EApply.
@@ -16,19 +17,14 @@ Set Strict Implicit.
 Section parameterized.
   Variable typ : Type.
   Variable expr : Type.
-  Variable subst : Type.
 
   Context {RType_typ : RType typ}.
+  Context {RTypeOk_typ : RTypeOk}.
   Context {Expr_expr : Expr RType_typ expr}.
+  Context {ExprOk_expr : ExprOk Expr_expr}.
   Context {Typ0_Prop : Typ0 _ Prop}.
-  Context {Subst_subst : Subst subst expr}.
-  Context {SubstOk_subst : @SubstOk _ _ _ _ Expr_expr Subst_subst}.
-  Context {SU : SubstUpdate subst expr}.
-  Context {SubstUpdateOk_subst : @SubstUpdateOk _ _ _ _ Expr_expr Subst_subst _ _}.
-  Context {SubstInstantiatable_subst : SubstInstantiatable subst expr}.
-  Context {SubstInstantiatableOk_subst : @SubstInstantiatableOk _ _ _ _ Expr_expr Subst_subst _ _}.
+  Context {ExprUVar_expr : ExprUVar expr}.
 
-  Variable UVar : nat -> expr.
   Variable vars_to_uvars : nat -> nat -> expr -> expr.
   Variable exprUnify : forall subst, Subst subst expr -> SubstUpdate subst expr ->
     tenv typ -> tenv typ -> nat -> expr -> expr -> typ -> subst -> option subst.
@@ -36,16 +32,16 @@ Section parameterized.
 
   Variable lem : Lemma.lemma typ expr expr.
 
-  Definition APPLY : rtac typ expr subst :=
-    @EAPPLY typ expr subst _ _ _ _ _ UVar vars_to_uvars exprUnify instantiate lem.
+  Definition APPLY : rtac typ expr :=
+    @EAPPLY typ expr _ _ _ vars_to_uvars exprUnify instantiate lem.
 
   Hypothesis lemD :
     @Lemma.lemmaD typ expr _ _ expr (@exprD'_typ0 _ _ _ _ Prop _)
                   _ nil nil lem.
 
-  Theorem APPLY_sound : rtac_sound nil nil APPLY.
+  Theorem APPLY_sound : rtac_sound APPLY.
   Proof.
-    eapply EAPPLY_sound.
+    eapply EAPPLY_sound; eauto.
   Qed.
 
 End parameterized.
